{
  "nbformat": 4,
  "nbformat_minor": 0,
  "metadata": {
    "colab": {
      "name": "probability_generating_functions.ipynb",
      "provenance": []
    },
    "kernelspec": {
      "name": "python3",
      "display_name": "Python 3"
    },
    "language_info": {
      "name": "python"
    }
  },
  "cells": [
    {
      "cell_type": "markdown",
      "metadata": {
        "id": "7Lmn0XYm_UEV"
      },
      "source": [
        "[![Open In Colab](https://colab.research.google.com/assets/colab-badge.svg)](https://colab.research.google.com/drive/1SeLHDzV-XWyOMSFIsRkDbRlTGM23cr4c?usp=sharing)"
      ]
    },
    {
      "cell_type": "markdown",
      "metadata": {
        "id": "Poeb8tYErDSN"
      },
      "source": [
        "#Probability Generating Functions (PGFs):\n",
        "\n",
        "The PGF of a discrete random variable (r.v.) is a power series representation of the probability mass function (PMF) of the r.v. A PGF lets us encode the sequence of probabilities $P(X = k)$ in the PMF of the r.v. into a continuous function (the PGF). We can now use tools from calculus to manipulate the PGF.\n",
        "\n",
        "**Definition:** Let $X$ be a discrete r.v. taking values in the non-negative integers $\\{0, 1, 2, . . .\\}$ with PMF $p(k) = P(X = k)$. The PGF of $X$ is:\n",
        "\n",
        "$$\\begin{eqnarray}\n",
        "G_X(s) &=& \\mathbb{E}(s^X)\\\\ \n",
        "&=& \\sum_{k = 0}^{\\infty}P(X = k)s^k \\\\\n",
        "&=& P(X = 0)s^0 + P(X = 1)s^1 + P(X = 2)s^2 + P(X = 3)s^3 + P(X = 4)s^4 + \\ldots\n",
        "\\end{eqnarray}$$\n",
        "\n",
        "Let's construct a PGF with the probabilities associated with the different outcomes of throwing a fair die.\n",
        "\n",
        "$$\\begin{eqnarray}\n",
        "G_X(s) &=& P(X = 0)s^0 + P(X = 1)s^1 + P(X = 2)s^2 + P(X = 3)s^3 + P(X = 4)s^4 + P(X = 5)s^5 + P(X = 6)s^6\\\\\n",
        "&=& 0s^0 + \\frac{1}{6}s^1 + \\frac{1}{6}s^2 + \\frac{1}{6}s^3 + \\frac{1}{6}s^4 + \\frac{1}{6}s^5 + \\frac{1}{6}s^6\n",
        "\\end{eqnarray}$$\n",
        "\n",
        "Note that $P(X = 0) = 0$ since \"$0$\" is not part of the possible outcomes of our fair die.\n",
        "\n",
        "##Properties of PGFs:\n",
        "\n",
        "1. $G_X(0) = P(X = 0)$\n",
        "  \n",
        "  Proof:\n",
        "\n",
        "$$\\begin{eqnarray}\n",
        "G_X(0) &=& P(X = 0)0^0 + P(X = 1)0^1 + P(X = 2)0^2 + P(X = 3)0^3 + P(X = 4)0^4 + \\ldots\\\\\n",
        "&=& P(X = 0)1 + P(X = 1)0 + P(X = 2)0 + P(X = 3)0 + P(X = 4)0 + \\ldots\\\\\n",
        "&=& P(X = 0)\n",
        "\\end{eqnarray}$$\n",
        "\n",
        "\n",
        "\n",
        "\n",
        "2. $G_X(1) = 1$\n",
        "\n",
        "  Proof:\n",
        "\n",
        "$$\\begin{eqnarray}\n",
        "G_X(1) &=& P(X = 0)1^0 + P(X = 1)1^1 + P(X = 2)1^2 + P(X = 3)1^3 + P(X = 4)1^4 + \\ldots\\\\\n",
        "&=& P(X = 0)1 + P(X = 1)1 + P(X = 2)1 + P(X = 3)1 + P(X = 4)1 + \\ldots\\\\\n",
        "&=& \\sum_{k = 0}^{\\infty}P(X = k) = 1\n",
        "\\end{eqnarray}$$\n",
        "\n",
        "\n",
        "Next, we can consider the first and second derivatives of $G_X(s)$ namely $G'_X(s)$ and $G''_X(s)$. The differentiation is with respect to $s$:\n",
        "\n",
        "$$\\begin{eqnarray}\n",
        "G'_X(s) &=& 0 + (1)P(X = 1)s^0 + (2)P(X = 2)s^1 + (3)P(X = 3)s^2 + (4)P(X = 4)s^3 + \\ldots\\\\\n",
        "G''_X(s) &=& 0 + 0 + (2)(1)P(X = 2)s^0 + (3)(2)P(X = 3)s^1 + (4)(3)P(X = 4)s^2 + \\ldots\n",
        "\\end{eqnarray}$$\n",
        "\n",
        "(We use the power rule: $\\frac{d}{ds}[s^n] = ns^{n-1}$, and the fact that: $\\frac{d}{ds}[s^0] = 0$ because $s^0$ is a constant.)\n",
        "\n",
        "We will also need to use the generalization of expectation of an arbitrary function of a random variable: $\\mathbb{E}[f(X)] = \\sum_{k=0}^{\\infty} f(k)P(X = k)$:\n",
        "\n",
        "\n",
        "3. $G'_X(1) = \\mathbb{E}[X]$\n",
        "\n",
        "  Proof:\n",
        "\n",
        "$$\\begin{eqnarray}\n",
        "G'_X(1) &=& 0 + (1)P(X = 1)1^0 + (2)P(X = 2)1^1 + (3)P(X = 3)1^2 + (4)P(X = 4)1^3 + \\ldots\\\\\n",
        "&=& (1)P(X = 1) + (2)P(X = 2) + (3)P(X = 3) + (4)P(X = 4) + \\ldots\\\\\n",
        "&=& \\sum_{k = 0}^{\\infty}kP(X = k) = \\mathbb{E}[X]\n",
        "\\end{eqnarray}$$\n",
        "\n",
        "\n",
        "4. $G''_X(1) = \\mathbb{E}[X^2] - \\mathbb{E}[X]$\n",
        "\n",
        "  Proof:\n",
        "\n",
        "$$\\begin{eqnarray}\n",
        "G''_X(s) &=& 0 + 0 + (2)(1)P(X = 2)1^0 + (3)(2)P(X = 3)1^1 + (4)(3)P(X = 4)1^2 + \\ldots\\\\\n",
        "&=& (2)(1)P(X = 2) + (3)(2)P(X = 3) + (4)(3)P(X = 4 + \\ldots\\\\\n",
        "&=& \\sum_{k = 0}^{\\infty}(k)(k-1)P(X = k) = \\mathbb{E}[X(X-1)]\\\\\n",
        "&=& \\mathbb{E}[X^2-X] = \\mathbb{E}[X^2] - \\mathbb{E}[X]\n",
        "\\end{eqnarray}$$\n",
        "\n",
        "\n",
        "5. $G''_X(1) + G'_X(1) - (G'_X(1))^2 =  \\mathbb{E}[(X - \\mathbb{E}[X])^2] = \\mathrm{Var}(X) $\n",
        "  Proof:\n",
        "\n",
        "$$\\begin{eqnarray}\n",
        "G''_X(1) + G'_X(1) - (G'_X(1))^2 &=& \\mathbb{E}[X^2] - \\mathbb{E}[X] + \\mathbb{E}[X] - (\\mathbb{E}[X])^2\\\\\n",
        "&=& \\mathbb{E}[X^2] - (\\mathbb{E}[X])^2\\\\\n",
        "&=& \\mathbb{E}[X^2] - (\\mathbb{E}[X])^2 + (\\mathbb{E}[X])^2 - (\\mathbb{E}[X])^2\\\\\n",
        "&=& \\mathbb{E}[X^2] - 2(\\mathbb{E}[X])^2 + (\\mathbb{E}[X])^2\\\\\n",
        "&=& \\mathbb{E}[X^2] -(2\\mathbb{E}[X])(\\mathbb{E}[X]) + (\\mathbb{E}[X])^2\\\\\n",
        "&=& \\mathbb{E}[X^2] -\\mathbb{E}[(2\\mathbb{E}[X])(X)] + \\mathbb{E}[(\\mathbb{E}[X])^2]\\\\\n",
        "&=&\\mathbb{E}[X^2 -(2\\mathbb{E}[X])(X) + (\\mathbb{E}[X])^2 ]\\\\\n",
        "&=&\\mathbb{E}[(X -\\mathbb{E}[X])^2]\\\\\n",
        "&=&\\mathrm{Var}(X)\n",
        "\\end{eqnarray}$$\n",
        "\n",
        "It is natural to ask, \"what is the interpretation of $s$ in $G_X(s)$? The answer is that $s$ does not have any interpretation in particular; it is just a device we introduce that allows us to manipulate our probabilities according to the rules of calculus. \n",
        "\n",
        "\n",
        "\n",
        "\n",
        "\n",
        "\n",
        "\n"
      ]
    }
  ]
}